TSO axiom: change axioms
- replace internal with cowr and corw
  (closes #21)
- update proofs
- leave some admits and check messages to be reviewed

Signed-off-by: Kyeongmin Cho <kyeongmin.cho@kaist.ac.kr>

src/axiomatic/TsoAxiomatic.v
@@ -523,11 +523,21 @@ Module Execution.
   .
   Hint Constructors label_loc.
 
+  Lemma label_is_mon
+        exec p1 p2 eid
+        (PREL: p1 <1= p2)
+        (P1: label_is exec p1 eid):
+    label_is exec p2 eid.
+  Proof.
+    destruct P1; eauto.
+  Qed.
+
   (* let obs = rfe | fr | co *)
-  (* let dob = ([W U U U R]; po; [W U U U R]) \ (W * R) *)
-  (* let bob = [E]; po; [MF]; po; [E] ~~~> [W]; po; [dmb wr]; po; [R]*)
+  (* let dob = ([R]; po; [E]) U ([E]; po; [W]) *)
+  (* let bob = [E]; po; [MF]; po; [E] ~~~> [W]; po; [dmb wr]; po; [R] *)
   (* let ob = obs | dob | bob *)
-  (* acyclic po-loc | fr as internal *)
+  (* irrefl po; rf as corw*)
+  (* irrefl po; fr as cowr *)
   (* acyclic ob as external *)
 
   Inductive po (eid1 eid2:eidT): Prop :=
@@ -574,6 +584,12 @@ Module Execution.
     econs 2. ss.
   Qed.
 
+  Lemma po_chain: Execution.po ⨾ Execution.po^? ⊆ Execution.po.
+  Proof.
+    ii. inv H. des. inv H0. destruct x, x0, y. ss. subst.
+    inv H1; inv H; ss. subst. econs; ss. lia.
+  Qed.
+
   Inductive i (eid1 eid2:eidT): Prop :=
   | i_intro
       (TID: fst eid1 = fst eid2)
@@ -586,7 +602,6 @@ Module Execution.
   .
   Hint Constructors e.
 
-  Definition po_loc (ex:t): relation eidT := po ∩ ex.(label_rel) label_loc.
   Definition fr (ex:t): relation eidT :=
     (ex.(rf)⁻¹ ⨾ ex.(co)) ∪
     ((ex.(label_rel) label_loc) ∩
@@ -594,27 +609,25 @@ Module Execution.
 
   Definition rfe (ex:t): relation eidT := ex.(rf) ∩ e.
 
-  Definition internal (ex:t): relation eidT := (po_loc ex) ∪ (fr ex).
+  Definition cowr (ex:t): relation eidT := po ⨾ (fr ex).
+  Definition corw (ex:t): relation eidT := po ⨾ ex.(rf).
 
   Definition obs (ex:t): relation eidT := (rfe ex) ∪ (fr ex) ∪ ex.(co).
 
-  (*
-   * CHECK: update는 (W*R)의 W에 들어올 수 없으므로
-   *        is_write에 update 넣을지 판단할 때 주의
-   *)
   Definition dob (ex:t): relation eidT :=
+    (⦗ex.(label_is) Label.is_read⦘ ⨾
+     po ⨾
+     ⦗ex.(label_is) Label.is_access⦘) ∪
     (⦗ex.(label_is) Label.is_access⦘ ⨾
      po ⨾
-     ⦗ex.(label_is) Label.is_access⦘)
-    \
-    (ex.(label_is) Label.is_write) × (ex.(label_is) Label.is_read).
+     ⦗ex.(label_is) Label.is_write⦘).
 
   Definition bob (ex:t): relation eidT :=
-    (⦗ex.(label_is) Label.is_write⦘ ⨾
+    ⦗ex.(label_is) Label.is_write⦘ ⨾
      po ⨾
      ⦗ex.(label_is) (Label.is_barrier_c Barrier.is_dmb_wr)⦘ ⨾
      po ⨾
-     ⦗ex.(label_is) Label.is_read⦘).
+     ⦗ex.(label_is) Label.is_read⦘.
 
   Definition ob (ex:t): relation eidT :=
     (obs ex) ∪ (dob ex) ∪ (bob ex).
@@ -661,35 +674,31 @@ Module Valid.
 
   Definition co1 (ex: Execution.t) :=
     forall eid1 eid2,
-      (exists loc
-          val1
-          val2,
-          <<LABEL: Execution.label eid1 ex = Some (Label.write loc val1)>> /\
-          <<LABEL: Execution.label eid2 ex = Some (Label.write loc val2)>>) ->
+      (exists loc,
+          <<LABEL: ex.(Execution.label_is) (Label.is_writing loc) eid1>> /\
+          <<LABEL: ex.(Execution.label_is) (Label.is_writing loc) eid2>>) ->
       (eid1 = eid2 \/ ex.(Execution.co) eid1 eid2 \/ ex.(Execution.co) eid2 eid1).
 
   Definition co2 (ex: Execution.t) :=
     forall eid1 eid2,
       ex.(Execution.co) eid1 eid2 ->
-      exists loc
-         val1
-         val2,
-        <<LABEL: Execution.label eid1 ex = Some (Label.write loc val1)>> /\
-        <<LABEL: Execution.label eid2 ex = Some (Label.write loc val2)>>.
+      exists loc,
+        <<LABEL: ex.(Execution.label_is) (Label.is_writing loc) eid1>> /\
+        <<LABEL: ex.(Execution.label_is) (Label.is_writing loc) eid2>>.
 
   Definition rf1 (ex: Execution.t) :=
     forall eid1 loc val
-       (LABEL: Execution.label eid1 ex = Some (Label.read loc val)),
+       (LABEL: ex.(Execution.label_is) (Label.is_reading_val loc val) eid1),
       (<<NORF: ~ codom_rel ex.(Execution.rf) eid1>> /\ <<VAL: val = Val.default>>) \/
       (exists eid2,
-          <<LABEL: Execution.label eid2 ex = Some (Label.write loc val)>> /\
+          <<LABEL: ex.(Execution.label_is) (Label.is_writing_val loc val) eid2>> /\
           <<RF: ex.(Execution.rf) eid2 eid1>>).
 
   Definition rf2 (ex: Execution.t) :=
     forall eid1 eid2 (RF: ex.(Execution.rf) eid2 eid1),
     exists loc val,
-      <<READ: Execution.label eid1 ex = Some (Label.read loc val)>> /\
-      <<WRITE: Execution.label eid2 ex = Some (Label.write loc val)>>.
+      <<READ: ex.(Execution.label_is) (Label.is_reading_val loc val) eid1>> /\
+      <<WRITE: ex.(Execution.label_is) (Label.is_writing_val loc val) eid2>>.
 
   Definition rf_wf (ex: Execution.t) := functional (ex.(Execution.rf))⁻¹.
 
@@ -700,7 +709,8 @@ Module Valid.
     RF1: rf1 ex;
     RF2: rf2 ex;
     RF_WF: rf_wf ex;
-    INTERNAL: acyclic (Execution.internal ex);
+    COWR: irreflexive (Execution.cowr ex);
+    CORW: irreflexive (Execution.corw ex);
     EXTERNAL: acyclic (Execution.ob ex);
   }.
   Hint Constructors ex.
@@ -740,40 +750,13 @@ Module Valid.
     inv EX. eapply po_label_pre; eauto.
   Qed.
 
-  Lemma coherence_rw
-        p exec
-        eid1 eid2 eid3 loc
-        (EX: ex p exec)
-        (EID1: exec.(Execution.label_is) (Label.is_reading loc) eid1)
-        (EID2: exec.(Execution.label_is) (Label.is_writing loc) eid2)
-        (EID3: exec.(Execution.label_is) (Label.is_writing loc) eid3)
-        (RF1: exec.(Execution.rf) eid3 eid1)
-        (PO: Execution.po eid1 eid2):
-    exec.(Execution.co) eid3 eid2.
+  Global Program Instance clos_refl_reflexive A R: Reflexive (@clos_refl A R).
+
+  Lemma po_irrefl:
+    forall eid,
+      ~ Execution.po eid eid.
   Proof.
-    inv EID1. apply Label.is_reading_inv in LABEL. des. subst.
-    inv EID2. apply Label.is_writing_inv in LABEL. des. subst.
-    inv EID3. apply Label.is_writing_inv in LABEL. des. subst.
-    exploit EX.(CO1).
-    { rewrite EID0, EID1. esplits; eauto. }
-    i. des.
-    - subst. exfalso. eapply EX.(INTERNAL). econs 2; econs.
-      + left. econs; eauto. econs; eauto.
-        econs; eauto using Label.read_is_accessing, Label.write_is_accessing.
-      + admit.
-      (* + left. econs; eauto. *)
-      (*   *  *)
-      (*   * econs; eauto using Label.read_is_accessing, Label.write_is_accessing. *)
-    - exfalso. eapply EX.(INTERNAL). econs 2; [econs|econs 2; econs].
-      + left. econs; eauto. econs; eauto.
-        econs; eauto using Label.read_is_accessing, Label.write_is_accessing.
-      + admit.
-      (* + left. right. eauto. *)
-      + admit.
-      (* + right. eauto. *)
-    - ss.
-  Grab Existential Variables.
-  { admit. (* will be gone automatically.. *) }
+    ii. inv H. lia.
   Qed.
 
   Lemma coherence_ww
@@ -785,18 +768,56 @@ Module Valid.
         (PO: Execution.po eid1 eid2):
     exec.(Execution.co) eid1 eid2.
   Proof.
-    inv EID1. apply Label.is_writing_inv in LABEL. des. subst.
-    inv EID2. apply Label.is_writing_inv in LABEL. des. subst.
-    exploit EX.(CO1).
-    { rewrite EID, EID0. esplits; eauto. }
+    inv EID1. inv EID2. exploit EX.(CO1).
+    { esplits; econs; [exact EID| |exact EID0|]; eauto. }
+    i. des; ss.
+    - subst. apply po_irrefl in PO. inv PO.
+    - exfalso. eapply EX.(EXTERNAL). apply t_step_rt. esplits.
+      + left. left. right. eauto.
+      + econs. left. right. right. econs. esplits.
+        * econs; eauto. econs; eauto using Label.writing_is_access.
+        * econs. esplits; eauto. econs; eauto. econs; eauto using Label.writing_is_write.
+  Qed.
+
+  Lemma coherence_wr
+        p exec
+        eid1 eid2 loc
+        (EX: ex p exec)
+        (EID1: exec.(Execution.label_is) (Label.is_writing loc) eid1)
+        (EID2: exec.(Execution.label_is) (Label.is_reading loc) eid2)
+        (PO: Execution.po eid1 eid2):
+    exists eid3,
+      <<RF: exec.(Execution.rf) eid3 eid2>> /\
+      <<CO: exec.(Execution.co)^? eid1 eid3>>.
+  Proof.
+    inv EID1. inv EID2. (* TODO: 기존에는 여기서 is_reading_inv를 사용하여 val을 얻었습니다 *)
+    exploit EX.(RF1).
+    { instantiate (1 := eid2). econs; eauto. instantiate (2 := loc).
+      (* TODO: is_reading으로부터 is_reading_val을 얻어야 하는데
+               여기서 val을 instantiate 할 수가 없습니다. *)
+      admit. }
     i. des.
-    - subst. inv PO. lia.
-    - ss.
-    - exfalso. eapply EX.(INTERNAL). econs 2; econs.
-      + left. econs; eauto. econs; eauto.
-        econs; eauto using Label.read_is_accessing, Label.write_is_accessing.
-      + admit.
-      (* + left. right. eauto. *)
+    { exfalso. eapply EX.(COWR). econs; econs.
+      - eauto.
+      - right. econs; eauto.
+        + econs; eauto.
+          econs; eauto using Label.writing_is_accessing, Label.reading_is_accessing.
+        + econs; econs; eauto using Label.reading_is_read, Label.writing_is_write.
+    }
+    esplits; eauto.
+    exploit EX.(CO1).
+    { esplits; [eauto|].
+      eapply Execution.label_is_mon; eauto. s. i.
+      eapply Label.writing_val_is_writing. eauto.
+    }
+    i. des; subst; ss.
+    { refl. }
+    { econs 2. ss. }
+    exfalso. eapply EX.(COWR). econs; econs.
+    - eauto.
+    - econs; eauto. econs; eauto.
+  Grab Existential Variables.
+    { admit. }
   Qed.
 
   Lemma coherence_rr
@@ -812,78 +833,103 @@ Module Valid.
       <<RF: exec.(Execution.rf) eid4 eid2>> /\
       <<CO: exec.(Execution.co)^? eid3 eid4>>.
   Proof.
-    inv EID1. apply Label.is_reading_inv in LABEL. des. subst.
-    inv EID2. apply Label.is_reading_inv in LABEL. des. subst.
-    inv EID3. apply Label.is_writing_inv in LABEL. des. subst.
-    exploit EX.(RF1); eauto. i. des.
-    { exfalso. eapply EX.(INTERNAL). econs 2; [econs|econs 2; econs].
-      - left. econs; eauto. econs; eauto.
-        econs; eauto using Label.read_is_accessing, Label.write_is_accessing.
-      - admit.
-        (* - right. eauto. *)
-      - admit.
-      (* - left. left. left. econs; eauto. econs; eauto. *)
-      (*   econs; eauto using Label.read_is_accessing, Label.write_is_accessing. *)
-    }
-    esplits; eauto.
-    exploit EX.(CO1).
-    { rewrite EID1, LABEL. esplits; eauto. }
-    i. des.
-    - subst. eauto.
-    - econs 2. ss.
-    - exfalso. eapply EX.(INTERNAL). econs 2; [econs|econs 2; econs].
-      + left. econs; eauto. econs; eauto.
-        econs; eauto using Label.read_is_accessing, Label.write_is_accessing.
-      + admit.
-        (* + left. left. right. left. econs; eauto. *)
-      + admit.
-      (* + right. ss. *)
-  Grab Existential Variables.
-  { admit. (* will be gone automatically.. *) }
-  { admit. (* will be gone automatically.. *) }
+    (* TODO *)
+    (* (1): exploit EX.(RF1) *)
+    (* (2): exploit EX.(CO1) *)
+    (* (3): contradiction of po; fr; rf
+            case rfe => ob "eid3 --rfe--> eid1 --co(from po)--> eid2 --fr--> eid3"
+            case rfi => cowr "eid3 --po(from rfi)--> eid1 --po--> eid2 --fr--> eid3"
+            *)
+    admit.
   Qed.
 
-  Lemma coherence_wr
+  (*   inv EID1. apply Label.is_reading_inv in LABEL. des. subst. *)
+  (*   inv EID2. apply Label.is_reading_inv in LABEL. des. subst. *)
+  (*   inv EID3. apply Label.is_writing_inv in LABEL. des. subst. *)
+  (*   exploit EX.(RF1); eauto. i. des. *)
+  (*   { exfalso. eapply EX.(INTERNAL). econs 2; [econs|econs 2; econs]. *)
+  (*     - left. econs; eauto. econs; eauto. *)
+  (*       econs; eauto using Label.read_is_accessing, Label.write_is_accessing. *)
+  (*     - admit. *)
+  (*       (* - right. eauto. *) *)
+  (*     - admit. *)
+  (*     (* - left. left. left. econs; eauto. econs; eauto. *) *)
+  (*     (*   econs; eauto using Label.read_is_accessing, Label.write_is_accessing. *) *)
+  (*   } *)
+  (*   esplits; eauto. *)
+  (*   exploit EX.(CO1). *)
+  (*   { rewrite EID1, LABEL. esplits; eauto. } *)
+  (*   i. des. *)
+  (*   - subst. eauto. *)
+  (*   - econs 2. ss. *)
+  (*   - exfalso. eapply EX.(INTERNAL). econs 2; [econs|econs 2; econs]. *)
+  (*     + left. econs; eauto. econs; eauto. *)
+  (*       econs; eauto using Label.read_is_accessing, Label.write_is_accessing. *)
+  (*     + admit. *)
+  (*       (* + left. left. right. left. econs; eauto. *) *)
+  (*     + admit. *)
+  (*     (* + right. ss. *) *)
+  (* Grab Existential Variables. *)
+  (* { admit. (* will be gone automatically.. *) } *)
+  (* { admit. (* will be gone automatically.. *) } *)
+  (* Qed. *)
+
+  Lemma coherence_rw
         p exec
-        eid1 eid2 loc
+        eid1 eid2 eid3 loc
         (EX: ex p exec)
-        (EID1: exec.(Execution.label_is) (Label.is_writing loc) eid1)
-        (EID2: exec.(Execution.label_is) (Label.is_reading loc) eid2)
+        (EID1: exec.(Execution.label_is) (Label.is_reading loc) eid1)
+        (EID2: exec.(Execution.label_is) (Label.is_writing loc) eid2)
+        (EID3: exec.(Execution.label_is) (Label.is_writing loc) eid3)
+        (RF1: exec.(Execution.rf) eid3 eid1)
         (PO: Execution.po eid1 eid2):
-    exists eid3,
-      <<RF: exec.(Execution.rf) eid3 eid2>> /\
-      <<CO: exec.(Execution.co)^? eid1 eid3>>.
+    exec.(Execution.co) eid3 eid2.
   Proof.
-    inv EID1. apply Label.is_writing_inv in LABEL. des. subst.
-    inv EID2. apply Label.is_reading_inv in LABEL. des. subst.
-    exploit EX.(RF1); eauto. i. des.
-    { exfalso. eapply EX.(INTERNAL). econs 2; econs.
-      - left. econs; eauto.
-        econs; eauto using Label.read_is_accessing, Label.write_is_accessing.
-      - admit.
-      (* - left. left. left. econs; eauto. econs; eauto. *)
-      (*   econs; eauto using Label.read_is_accessing, Label.write_is_accessing. *)
-    }
-    esplits; eauto.
+    inv EID1. inv EID2. inv EID3.
     exploit EX.(CO1).
-    { rewrite EID, LABEL. esplits; eauto. }
-    i. des.
-    - subst. eauto.
-    - econs 2. ss.
-    - exfalso. eapply EX.(INTERNAL). econs 2; econs.
-      + left. econs; eauto. econs; eauto.
-        econs; eauto using Label.read_is_accessing, Label.write_is_accessing.
-      + admit.
-      (* + left. left. right. left. econs; eauto. *)
+    { esplits; econs; [exact EID0| |exact EID1|]; eauto. }
+    i. apply or_assoc in x0. destruct x0; [|done].
+    destruct (fst eid1 == fst eid3).
+    - (* rfi *)
+      exfalso. eapply EX.(CORW). econs; eauto. esplits; [|by eauto].
+      apply Execution.po_chain. econs. splits; eauto.
+      des; [by left|right].
+      destruct eid1 as [tid1 iid1].
+      destruct eid2 as [tid2 iid2].
+      destruct eid3 as [tid3 iid3].
+      inv e. inversion PO. ss. subst.
+      destruct (lt_eq_lt_dec iid3 iid2); ss.
+      exfalso. eapply EX.(EXTERNAL). apply t_step_rt. esplits.
+      { left. left. right. eauto. }
+      destruct s.
+      + econs 1. left. right. right. econs. esplits.
+        * econs; eauto. econs; eauto using Label.writing_is_access.
+        * econs. esplits; cycle 1.
+          { econs; eauto. econs; eauto using Label.writing_is_write. }
+          eauto.
+      + subst. econs 2.
+    - (* rfe *)
+      exfalso. eapply EX.(EXTERNAL). apply t_step_rt. esplits.
+      { inversion H.
+        - left. left. left. left. econs; eauto.
+        - left. left. left. left. econs; eauto.
+      }
+      etrans.
+      + instantiate (1 := eid2). econs. left. right. left. econs. econs.
+        * econs; eauto. econs; eauto using Label.reading_is_read.
+        * econs; eauto. econs; eauto. econs; eauto. econs; eauto using Label.writing_is_access.
+      + econs. inversion H.
+        * exfalso. inv PO. eauto.
+        * left. left. right. eauto.
   Qed.
 
   Lemma rf_inv_write
         p exec
         eid1 eid2 loc val
         (EX: ex p exec)
-        (EID2: Execution.label eid2 exec = Some (Label.read loc val))
+        (EID2: exec.(Execution.label_is) (Label.is_reading_val loc val) eid2)
         (RF3: exec.(Execution.rf) eid1 eid2):
-    <<LABEL: Execution.label eid1 exec = Some (Label.write loc val)>>.
+    <<LABEL: exec.(Execution.label_is) (Label.is_writing_val loc val) eid1>>.
   Proof.
     exploit EX.(RF1); eauto. i. des.
     - contradict NORF. econs. eauto.
@@ -924,10 +970,16 @@ Module Valid.
     inv EID1. destruct l; ss. unfold co2, rf2 in *.
     obtac; ss.
     all: try by etrans; eauto.
-    - exploit RF2; eauto. i. des. congr.
-    - exploit RF2; eauto. i. des. congr.
+    - exploit RF2; eauto. i. des. inv WRITE. inv READ.
+      destruct l; ss. destruct l0; ss. congr. congr.
+      destruct l0; ss. congr. congr.
+    - exploit RF2; eauto. i. des. inv WRITE. inv READ.
+      destruct l; ss. destruct l0; ss. congr. congr.
+      destruct l0; ss. congr. congr.
     - destruct l1; try congr; ss.
-    - exploit CO2; eauto. i. des. congr.
+    - exploit CO2; eauto. i. des. inv LABEL0. inv LABEL1.
+      destruct l; ss. destruct l0; ss. congr. congr.
+      destruct l0; ss. congr. congr.
   Qed.
 
   Lemma ob_barrier_ob
@@ -947,9 +999,15 @@ Module Valid.
     all: try by rewrite EID in EID1; inv EID1; ss.
     all: try by rewrite EID in EID2; inv EID2; ss.
     all: try by destruct l; try congr; ss.
-    - exploit RF2; eauto. i. des. congr.
-    - exploit CO2; eauto. i. des. congr.
-    - exploit CO2; eauto. i. des. congr.
+    - exploit RF2; eauto. i. des. inv WRITE. inv READ.
+      destruct l; ss. destruct l0; ss. congr. congr.
+      destruct l0; ss. congr. congr.
+    - exploit CO2; eauto. i. des. inv LABEL0. inv LABEL1.
+      destruct l; ss. destruct l0; ss. congr. congr.
+      destruct l0; ss. congr. congr.
+    - exploit CO2; eauto. i. des. inv LABEL0. inv LABEL1.
+      destruct l; ss. destruct l0; ss. congr. congr.
+      destruct l0; ss. congr. congr.
   Qed.
 
   Lemma ob_label
@@ -965,8 +1023,15 @@ Module Valid.
     unfold co2, rf2 in *.
     obtac.
     all: try congr.
-    all: try by exploit RF2; eauto; i; des; congr.
-    all: try by exploit CO2; eauto; i; des; congr.
+    - exploit RF2. eauto. i. des. inv WRITE. inv READ.
+      destruct l; ss. destruct l0; ss. congr. congr.
+      destruct l0; ss. congr. congr.
+    - exploit RF2. eauto. i. des. inv WRITE. inv READ.
+      destruct l; ss. destruct l0; ss. congr. congr.
+      destruct l0; ss. congr. congr.
+    - exploit CO2. eauto. i. des. inv LABEL. inv LABEL0.
+      destruct l; ss. destruct l0; ss. congr. congr.
+      destruct l0; ss. congr. congr.
   Qed.
 
   Lemma ob_cycle
@@ -994,46 +1059,49 @@ Module Valid.
       + exfalso. eapply ob_label; eauto.
   Qed.
 
-  Lemma internal_rw
-        p ex
-        eid1 eid2
-        (PRE: pre_ex p ex)
-        (CO2: co2 ex)
-        (RF2: rf2 ex)
-        (INTERNAL: Execution.internal ex eid1 eid2):
-    <<EID1: ex.(Execution.label_is) Label.is_access eid1>> /\
-    <<EID2: ex.(Execution.label_is) Label.is_access eid2>>.
-  Proof.
-    unfold Execution.internal in *. obtac.
-    - inv H. inv H1. inv LABEL. splits.
-      + destruct l1; ss; econs; eauto.
-      + destruct l2; ss; econs; eauto.
-    - exploit CO2; eauto. i. des.
-      exploit RF2; eauto. i. des.
-      splits; econs; eauto.
-    - splits.
-      + destruct l1; ss; econs; eauto.
-      + destruct l2; ss; econs; eauto.
-  Qed.
+  (* CHECK: 하는 것? *)
+  (* Lemma internal_rw *)
+  (*       p ex *)
+  (*       eid1 eid2 *)
+  (*       (PRE: pre_ex p ex) *)
+  (*       (CO2: co2 ex) *)
+  (*       (RF2: rf2 ex) *)
+  (*       (INTERNAL: Execution.internal ex eid1 eid2): *)
+  (*   <<EID1: ex.(Execution.label_is) Label.is_access eid1>> /\ *)
+  (*   <<EID2: ex.(Execution.label_is) Label.is_access eid2>>. *)
+  (* Proof. *)
+  (*   unfold Execution.internal in *. obtac. *)
+  (*   - inv H0. inv H1. inv LABEL. splits. *)
+  (*     + destruct l1; ss; econs; eauto. *)
+  (*     + destruct l2; ss; econs; eauto. *)
+  (*   - exploit CO2; eauto. i. des. *)
+  (*     exploit RF2; eauto. i. des. *)
+  (*     splits; econs; eauto. *)
+  (*   - splits. *)
+  (*     + destruct l1; ss; econs; eauto. *)
+  (*     + destruct l2; ss; econs; eauto. *)
+  (* Qed. *)
 
-  Lemma internal_read_read_po
-        p ex
-        eid1 eid2
-        (PRE: pre_ex p ex)
-        (CO2: co2 ex)
-        (RF2: rf2 ex)
-        (INTERNAL: Execution.internal ex eid1 eid2)
-        (EID1: ex.(Execution.label_is) Label.is_read eid1)
-        (EID2: ex.(Execution.label_is) Label.is_read eid2):
-    Execution.po eid1 eid2.
-  Proof.
-    unfold Execution.internal in *. obtac.
-    - inv H. ss.
-    - exploit CO2; eauto. i. des.
-      destruct l; ss. congr.
-    - rewrite EID in EID0. inv EID0. destruct l0; ss.
-  Qed.
+  (* CHECK: 하는 것? *)
+  (* Lemma internal_read_read_po *)
+  (*       p ex *)
+  (*       eid1 eid2 *)
+  (*       (PRE: pre_ex p ex) *)
+  (*       (CO2: co2 ex) *)
+  (*       (RF2: rf2 ex) *)
+  (*       (INTERNAL: Execution.internal ex eid1 eid2) *)
+  (*       (EID1: ex.(Execution.label_is) Label.is_read eid1) *)
+  (*       (EID2: ex.(Execution.label_is) Label.is_read eid2): *)
+  (*   Execution.po eid1 eid2. *)
+  (* Proof. *)
+  (*   unfold Execution.internal in *. obtac. *)
+  (*   - inv H. ss. *)
+  (*   - exploit CO2; eauto. i. des. *)
+  (*     destruct l; ss. congr. *)
+  (*   - rewrite EID in EID0. inv EID0. destruct l0; ss. *)
+  (* Qed. *)
 
+  (* CHECK: 하는 것? *)
   Lemma ob_read_read_po
         p ex
         eid1 eid2
@@ -1043,7 +1111,7 @@ Module Valid.
         (RF1: rf1 ex)
         (RF2: rf2 ex)
         (RF_WF: rf_wf ex)
-        (INTERNAL: acyclic (Execution.internal ex))
+        (* (INTERNAL: acyclic (Execution.internal ex)) *)
         (OB: Execution.ob ex eid1 eid2)
         (EID1: ex.(Execution.label_is) Label.is_read eid1)
         (EID2: ex.(Execution.label_is) Label.is_read eid2):
@@ -1052,41 +1120,49 @@ Module Valid.
     inv EID1. inv EID2. destruct l; ss. destruct l0; ss.
     unfold Execution.ob in *. obtac; try congr.
     all: try by etrans; eauto.
-    all: try by exploit RF2; eauto; i; des; congr.
-    all: try by exploit CO2; eauto; i; des; congr.
+    - exploit RF2. eauto. i. des. inv WRITE. inv READ.
+      destruct l; ss. destruct l0; ss. congr. congr.
+      destruct l0; ss. congr. congr.
+    - admit. (* r --fr--> r *)
     - inv H. rewrite EID0 in EID1. inv EID1. inv LABEL1.
+    - exploit CO2. eauto. i. des. inv LABEL1. inv LABEL2.
+      destruct l; ss. destruct l0; ss. congr. congr.
+      destruct l0; ss. congr. congr.
+    - admit. (* r --ob--> u *)
+    - admit. (* u --ob--> r,u *)
   Qed.
 
-  Lemma po_loc_write_is_co
-        ex eid1 eid2 loc
-        (CO1: Valid.co1 ex)
-        (INTERNAL: acyclic (Execution.internal ex))
-        (PO: Execution.po eid1 eid2)
-        (LABEL1: ex.(Execution.label_is) (Label.is_writing loc) eid1)
-        (LABEL2: ex.(Execution.label_is) (Label.is_writing loc) eid2):
-    ex.(Execution.co) eid1 eid2.
-  Proof.
-    destruct eid1 as [tid1 eid1], eid2 as [tid2 eid2].
-    inv LABEL1. inv LABEL2. destruct l, l0; ss.
-    destruct (equiv_dec loc0 loc) eqn:Heq1; ss.
-    destruct (equiv_dec loc1 loc) eqn:Heq2; ss.
-    rewrite e, e0 in *.
-    exploit CO1.
-    { esplits; [exact EID|exact EID0]. }
-    i. des; eauto.
-    - inv x. inv PO. ss. lia.
-    - exfalso. eapply INTERNAL. econs 2.
-      + econs 1. left. econs; eauto.
-        econs; eauto. econs; unfold Label.is_accessing; eauto.
-        * instantiate (1 := loc).
-          destruct (equiv_dec loc loc); ss.
-        * destruct (equiv_dec loc loc); ss.
-      + econs 1.
-        (* 원래는 internal을 쪼개서 Execution.co를 건지는데 여기는 co가 없음 *)
-        admit.
-        (* TODO: admit 없는 버전이랑 비교해서 없애기 *)
-        (* econs 1. left. right. eauto. *)
-  Qed.
+  (* CHECK: 하는 것? *)
+  (* Lemma po_loc_write_is_co *)
+  (*       ex eid1 eid2 loc *)
+  (*       (CO1: Valid.co1 ex) *)
+  (*       (INTERNAL: acyclic (Execution.internal ex)) *)
+  (*       (PO: Execution.po eid1 eid2) *)
+  (*       (LABEL1: ex.(Execution.label_is) (Label.is_writing loc) eid1) *)
+  (*       (LABEL2: ex.(Execution.label_is) (Label.is_writing loc) eid2): *)
+  (*   ex.(Execution.co) eid1 eid2. *)
+  (* Proof. *)
+  (*   destruct eid1 as [tid1 eid1], eid2 as [tid2 eid2]. *)
+  (*   inv LABEL1. inv LABEL2. destruct l, l0; ss. *)
+  (*   destruct (equiv_dec loc0 loc) eqn:Heq1; ss. *)
+  (*   destruct (equiv_dec loc1 loc) eqn:Heq2; ss. *)
+  (*   rewrite e, e0 in *. *)
+  (*   exploit CO1. *)
+  (*   { esplits; [exact EID|exact EID0]. } *)
+  (*   i. des; eauto. *)
+  (*   - inv x. inv PO. ss. lia. *)
+  (*   - exfalso. eapply INTERNAL. econs 2. *)
+  (*     + econs 1. left. econs; eauto. *)
+  (*       econs; eauto. econs; unfold Label.is_accessing; eauto. *)
+  (*       * instantiate (1 := loc). *)
+  (*         destruct (equiv_dec loc loc); ss. *)
+  (*       * destruct (equiv_dec loc loc); ss. *)
+  (*     + econs 1. *)
+  (*       원래는 internal을 쪼개서 Execution.co를 건지는데 여기는 co가 없음 *)
+  (*       admit. *)
+  (*       TODO: admit 없는 버전이랑 비교해서 없애기 *)
+  (*       econs 1. left. right. eauto. *)
+  (* Qed. *)
 End Valid.
 
 Coercion Valid.PRE: Valid.ex >-> Valid.pre_ex.
